src/npolynomial.lean
@@ -1,5 +1,6 @@
 import data.polynomial
 
+@[mono]
 lemma monotone_polynomial_nat (p : polynomial ℕ) : monotone (λ n : ℕ, p.eval n) :=
 begin
   induction p using polynomial.induction_on' with p q h₀ h₁ n a,
